theories/Dot/lr/lr_lemmasDefs.v
@@ -13,14 +13,14 @@ Section Sec.
   Local Arguments def_interp_vmem: simpl never. *)
 
   (** This lemma is equivalent to pDOT's (Def-New). *)
-  Lemma sD_New_Mem_I {Γ l ds} {T : ldslty Σ}:
-    oAnd (oLater (ldslty_olty T)) (oSing (pself (pv (ids 1)) l)) :: Γ s⊨ds ds : T -∗
-    Γ s⊨ { l := dpt (pv (vobj ds)) } : oLDVMem l (oMu (ldslty_olty T)).
+  Lemma sD_New_Mem_I {Γ l ds} {T : clty Σ}:
+    oAnd (oLater (clty_olty T)) (oSing (pself (pv (ids 1)) l)) :: Γ s⊨ds ds : T -∗
+    Γ s⊨ { l := dpt (pv (vobj ds)) } : oLDVMem l (oMu (clty_olty T)).
   Proof.
     iDestruct 1 as (Hwf) "#Hds";
       iIntros "!>" (ρ Hpid%path_includes_field_aliases) "#Hg".
     rewrite def_interp_tvmem_eq path_wp_pv /=. iLöb as "IH".
-    iApply ldslty_commute. rewrite norm_selfSubst.
+    iApply clty_commute. rewrite norm_selfSubst.
     iApply ("Hds" $! (vobj _ .: ρ) with "[%] [$IH $Hg //]").
     exact: path_includes_self.
   Qed.
@@ -50,13 +50,13 @@ Section Sec.
    * ---------------------
    * Γ ⊨ nu x. ds : μ x. T
    *)
-  Lemma sT_Obj_I (Γ : sCtx Σ) (T : ldslty Σ) ds:
-     oLater (ldslty_olty T) :: Γ s⊨ds ds : T -∗
-     Γ s⊨ tv (vobj ds) : oMu (ldslty_olty T).
+  Lemma sT_Obj_I (Γ : sCtx Σ) (T : clty Σ) ds:
+     oLater (clty_olty T) :: Γ s⊨ds ds : T -∗
+     Γ s⊨ tv (vobj ds) : oMu (clty_olty T).
   Proof.
     iDestruct 1 as (Hwf) "#Hds"; iIntros "!>" (ρ) "#Hg /= !>".
     rewrite -wp_value' /=. iLöb as "IH".
-    iApply ldslty_commute. rewrite norm_selfSubst.
+    iApply clty_commute. rewrite norm_selfSubst.
     iApply ("Hds" $! (vobj _ .: ρ) with "[%] [$IH $Hg]").
     exact: path_includes_self.
   Qed.
@@ -72,9 +72,9 @@ Section Sec.
   Lemma D_Nil Γ : Γ ⊨ds [] : TTop.
   Proof. apply sD_Nil. Qed.
 
-  Lemma sD_Cons Γ d ds l (T1 T2 : ldsltyO Σ):
+  Lemma sD_Cons Γ d ds l (T1 T2 : cltyO Σ):
     dms_hasnt ds l →
-    Γ s⊨ { l := d } : ldslty_dlty T1 -∗ Γ s⊨ds ds : T2 -∗
+    Γ s⊨ { l := d } : clty_dlty T1 -∗ Γ s⊨ds ds : T2 -∗
     Γ s⊨ds (l, d) :: ds : LDsAnd T1 T2.
   Proof.
     iIntros (Hlds) "#HT1 [% #HT2]"; iSplit.
@@ -82,8 +82,8 @@ Section Sec.
     iIntros "!>" (ρ [Hpid Hpids]%path_includes_split) "#Hg".
     iSpecialize ("HT1" $! _  Hpid with "Hg").
     iDestruct ("HT2" $! _  Hpids with "Hg") as "{HT2} HT2".
-    iSplit; first by iApply ldslty_def2defs_head.
-    iApply (ldslty_mono with "HT2"); by [apply dms_hasnt_subst | eapply nclosed_sub_app].
+    iSplit; first by iApply clty_def2defs_head.
+    iApply (clty_mono with "HT2"); by [apply dms_hasnt_subst | eapply nclosed_sub_app].
   Qed.
 
   Lemma D_Cons Γ d ds l T1 T2:
